factored out HaltL <= HaltLclosed from L_to_mTM

theories/TM/Reductions/L_to_mTM.v
@@ -2,10 +2,10 @@ Require Import Undecidability.TM.TM.
 Require Import Undecidability.Synthetic.Definitions Undecidability.Synthetic.ReducibilityFacts.
 From Undecidability.L Require Import L Seval LM_heap_def LM_heap_correct.
 Require Import Undecidability.TM.L.HeapInterpreter.M_LHeapInterpreter.
+Require Undecidability.L.Reductions.HaltL_to_HaltLclosed.
+Import HaltL_to_HaltLclosed (HaltLclosed).
 
 (* * L to TM *)
-
-Definition HaltLclosed (s : {s : term | closed s}) := exists t, eval (proj1_sig s) t. (* Halting problem for call-by-value lambda-calculus *)
 
 Definition eva_LM_lin sigma := exists tau, evaluates step sigma tau.
 
@@ -33,21 +33,6 @@ Proof.
   now eapply red_haltL_to_LM_Lin.
 Qed.
 
-Require Import Undecidability.L.Functions.Encoding Undecidability.L.Functions.Eval Undecidability.L.Tactics.LTactics.
-Import L_Notations.
-
-Lemma HaltL_HaltLclosed :
-  HaltL ⪯ HaltLclosed.
-Proof.
-  unshelve eexists.
-  - intros s. exists (Eval (enc s)). unfold Eval. Lproc. 
-  - cbn. intros s. unfold HaltL. split; intros (t & Ht).
-    + eapply eval_converges. edestruct Eval_converges. eapply H.
-      eapply eval_iff in Ht. eauto.
-    + setoid_rewrite eval_iff. eapply eval_converges. eapply Eval_converges. eapply Seval.eval_converges. eauto.
-Qed.
-
-
 Lemma star_def_equiv X R (x y : X):
   star R x y <-> Relations.star R x y.
 Proof.
@@ -65,7 +50,7 @@ Qed.
 Lemma HaltL_HaltTM :
   HaltL ⪯ HaltTM 11.
 Proof.
-  eapply reduces_transitive. 1:exact HaltL_HaltLclosed.
+  eapply reduces_transitive. 1:exact HaltL_to_HaltLclosed.reduction.
   eapply reduces_transitive. 1:exact LM_halting_LM_halting.
   eexists (fun x => (existT2 _ _ _ _ _)). intro.
   setoid_rewrite <- halts_eva_LM_lin.
